finite injury

src/tree_of_strategy.lean
@@ -14,53 +14,51 @@ inductive zero : Type
 
 def Tree' : ℕ → Type
 | 0       := zero
-| (n + 1) := list (Tree' n ⊕ infinity)
+| (n + 1) := list (infinity ⊕ Tree' n)
 
 instance : ∀ n, decidable_eq (Tree' n)
 | 0       := zero.decidable_eq
-| (n + 1) := @list.decidable_eq _ (@sum.decidable_eq _ (Tree'.decidable_eq n) infinity _)
+| (n + 1) := @list.decidable_eq _ (@sum.decidable_eq infinity _ _ (Tree'.decidable_eq n))
 
 def Tree (n : ℕ) := Tree' (n + 1)
 
-def subTree {n} (η : Tree n) := { μ : Tree n // μ <:+ η }
+def subTree {n} (η : Tree n) := { μ : Tree n // μ <:+ η ∧ μ ≠ η }
 
-def subTree.cons' {n} {η : Tree n} {a} (μ : subTree η) : subTree (a :: η) :=
-⟨μ.val, list.suffix_cons_iff.mpr(or.inr μ.property)⟩
+structure Tree_path (n : ℕ) :=
+(path : ℕ → Tree n)
+(ordered : ∀ m, path m <:+ path (m + 1))
 
-instance : has_zero (zero ⊕ infinity) := ⟨sum.inl zero.zero⟩
-instance {n} : has_emptyc (Tree n) := ⟨[]⟩
-
-notation `∞` := sum.inr infinity.infinity
-
-
-#check @list.rec_on
+@[simp] lemma list.cons_neq {α : Type*} (a : α) : ∀ (l : list α), l ≠ a :: l
+| [] := by simp
+| (a₁ :: l) := by { simp, intros h, simp[h], exact list.cons_neq l }
 
 
-
-@[elab_as_eliminator]
-theorem Tree'.rec_on {n} {motive : Tree' (n+1) → Sort*} (μ : Tree' (n + 1))
-  (nil : motive [])
-  (cons₁ : Π (ν : Tree' n) (μ : Tree' (n + 1)), motive μ → motive (sum.inl ν :: μ))
-  (cons₂ : Π (μ : Tree' (n + 1)), motive μ → motive (∞ :: μ)) : motive μ :=
+@[simp] lemma list.suffix_cons_append_left {α : Type*} (a : α) : ∀ (l₁ l₂ : list α), ¬ l₁ ++ a :: l₂ <:+ l₂ :=
 begin
-  induction μ with ν μ IH, refine nil,
-  cases ν, { refine cons₁ ν μ IH },
-  { cases ν, refine cons₂ μ IH }
+  intros l₁ l₂, induction l₂ with hd tl IH generalizing l₁ a,
+  { simp },
+  intros h, have := list.suffix_cons_iff.mp h, cases this,
+  { have lmm := (@list.append_left_inj _ (l₁ ++ [a]) [] (hd :: tl)), simp at lmm, exact lmm this },
+  { have IH := IH (l₁ ++ [a]) hd, simp at IH, exact IH this }
 end
 
-@[elab_as_eliminator]
-theorem Tree.rec_on {n} {motive : Tree (n+1) → Sort*} (μ : Tree (n + 1))
-  (nil : motive [])
-  (cons₁ : Π (ν : Tree n) (μ : Tree (n + 1)), motive μ → motive (sum.inl ν :: μ))
-  (cons₂ : Π (μ : Tree (n + 1)), motive μ → motive (∞ :: μ)) : motive μ :=
-@Tree'.rec_on (n + 1) motive μ nil cons₁ cons₂
+@[simp] lemma list.suffix_cons_left {α : Type*} (a : α) : ∀ (l : list α), ¬ a :: l <:+ l :=
+begin
+  suffices : ∀ (l₁ l₂ : list α), ¬a :: l₂ ++ l₁ <:+ l₁, { intros l, refine this l [] },
+  intros l₁, induction l₁ with hd tl IH,
+  { simp },
+  intros l₂ h, have := list.suffix_cons_iff.mp h, simp at*, cases this,
+  { have lmm := (@list.append_left_inj _ (l₂ ++ [hd]) [] tl), simp at lmm, exact lmm this.2 },
+  { have e : a :: (l₂ ++ hd :: tl) = ([a] ++ l₂ ++ [hd]) ++ tl, { simp }, rw e at this,
+    refine IH _ this }
+end
 
-@[elab_as_eliminator]
-theorem Tree'.rec_on₁ {motive : Tree 1 → Sort*} (μ : Tree 1) 
-  (nil : motive (∅ : Tree 1))
-  (cons₁ : Π (ν : Tree 0) (μ : Tree 1), motive μ → motive (sum.inl ν :: μ))
-  (cons₂ : Π (μ : Tree 1), motive μ → motive (∞ :: μ : Tree 1)) : motive μ :=
-@Tree'.rec_on 1 motive μ nil cons₁ cons₂
+def subTree.cons' {n} {η : Tree n} {a} (μ : subTree η) : subTree (a :: η) :=
+⟨μ.val, ⟨list.suffix_cons_iff.mpr (or.inr μ.property.1), λ h, by { have := μ.property.1, simp[h] at*, exact this }⟩⟩
+
+instance : has_zero (zero ⊕ infinity) := ⟨sum.inl zero.zero⟩
+
+notation `∞` := sum.inl infinity.infinity
 
 @[simp] def list.foldl' {α : Type*} (f : α → α → α) : list α → option α
 | []        := none
@@ -76,120 +74,136 @@ structure strategy (R : Type*) :=
 namespace strategy
 variables {R : Type*} (S : strategy R)
 
-@[reducible] def out {n} (μ η: Tree n) (ν : Tree' n ⊕ infinity) : Prop := ν :: μ <:+ η
+@[reducible] def out {n} (μ η: Tree n) (ν : infinity ⊕ Tree' n) : Prop := ν :: μ <:+ η
 notation `out[` η `] ` μ ` ↝ ` ν := out μ η ν
 
 namespace approx
 
-def weight (μ : Tree 1) : Π (η : Tree 0) (υ : subTree η → option (Tree 1)), ℕ
+def weight (μ : Tree 1) : Π {η : Tree 0} (υ : subTree η → option (Tree 1)), ℕ
 | []       _ := 0
-| (_ :: η) υ := weight η (λ ν, υ ν.cons') +
-  (if υ ⟨η, by simp⟩ = ↑μ then 1 else 0)
-
-/--
-def weight (η : Tree 1) : Tree 0 → ℕ
-| []       := 0
-| (_ :: μ) := weight μ + (if υ μ = ↑η then 1 else 0)
--/
+| (_ :: η) υ := @weight η (λ ν, υ ν.cons') + (if υ ⟨η, by simp⟩ = ↑μ then 1 else 0)
 
 def is_exists_inv_infinity (μ : Tree 1) :
-  Π (η : Tree 0) (υ : subTree η → option (Tree 1)), option (Tree 0)
+  Π {η : Tree 0} (υ : subTree η → option (Tree 1)), option (Tree 0)
 | []               _ := none
-| (sum.inl _ :: η) υ := is_exists_inv_infinity η (λ ν, υ ν.cons')
 | (∞ :: η)        υ :=
-    if (is_exists_inv_infinity η (λ ν, υ ν.cons')).is_some then
-      is_exists_inv_infinity η (λ ν, υ ν.cons') else
+    if (@is_exists_inv_infinity η (λ ν, υ ν.cons')).is_some then
+      @is_exists_inv_infinity η (λ ν, υ ν.cons') else
     if υ ⟨η, by simp⟩ = ↑μ then some η else none
+| (sum.inr _ :: η) υ := @is_exists_inv_infinity η (λ ν, υ ν.cons')
 
-#check is_exists_inv_infinity
-lemma is_exists_inv_infinity_infinity (η : Tree 1) (μ : Tree 0) (υ : subTree μ → option (Tree 1)) {μ₀ : Tree 0}
-  (h1 : out[μ] μ₀ ↝ ∞) (h2 : υ ⟨μ₀, by { sorry }⟩ = η) : (is_exists_inv_infinity η μ υ).is_some :=
+lemma out_subtree {n} {η μ : Tree n} {x} (h : out[η] μ ↝ x) : μ <:+ η ∧ μ ≠ η :=
+by { simp[out, list.is_suffix] at*, split,
+     { rcases h with ⟨ν, ν_p⟩, refine ⟨ν ++ [x], _⟩, simp* at* },
+     { intros e, rcases e with rfl, rcases h with ⟨ν, h⟩,
+       have := @list.append_left_inj _ (ν ++ [x]) [] μ, simp at this, exact this h } }
+
+lemma is_exists_inv_infinity_infinity (η : Tree 1) (μ : Tree 0) (υ : subTree μ → option (Tree 1)) (μ₀ : subTree μ)
+  (h1 : out[μ] μ₀.val ↝ ∞) (h2 : υ μ₀ = η) : (@is_exists_inv_infinity η μ υ).is_some :=
 begin
   induction μ with ν μ IH μ IH generalizing μ₀,
   { exfalso, simp[out] at*, exact h1 },
   cases ν,
+  { cases ν, simp[is_exists_inv_infinity] at*,
+    cases C : (@is_exists_inv_infinity η μ (λ ν, υ ν.cons')).is_some; simp[C],
+    { have : ∞ :: μ₀.val = ∞ :: μ ∨ out[μ] μ₀.val ↝ ∞, from list.suffix_cons_iff.mp h1,
+      cases this,
+      { simp at this, simp[←this, h2] },
+      { exfalso, have := IH (λ ν, υ ν.cons') ⟨μ₀.val, out_subtree this⟩ this (by simp[subTree.cons']; exact h2),
+        exact bool_iff_false.mpr C this } } },
   { simp[is_exists_inv_infinity],
-    have : ∞ :: μ₀ = sum.inl ν :: μ ∨ out[μ] μ₀ ↝ ∞, from list.suffix_cons_iff.mp h1,
+    have : ∞ :: μ₀.val = sum.inr ν :: μ ∨ out[μ] μ₀.val ↝ ∞, from list.suffix_cons_iff.mp h1,
     cases this,
     { simp at*, exfalso, exact this },
-    { refine IH this h2 } },
-  { cases ν, simp[is_exists_inv_infinity] at*,
-    cases C : (is_exists_inv_infinity υ η μ).is_some; simp[C],
-    { have : ∞ :: μ₀ = ∞ :: μ ∨ out[μ] μ₀ ↝ ∞, from list.suffix_cons_iff.mp h1,
-      cases this,
-      { simp at*, rcases this with rfl, simp[h2] },
-      { exfalso, have := IH this h2, exact bool_iff_false.mpr C this } } }
+    { simp at*, have := IH (λ ν, υ ν.cons') ⟨μ₀.val, out_subtree this⟩ this (by simp[subTree.cons']; exact h2),
+      exact this } }
 end
 
-def lambda' (η : Tree 0) (υ : subTree η → option (Tree 1)) : ℕ → Tree 1
+def lambda' {η : Tree 0} (υ : subTree η → option (Tree 1)) : ℕ → Tree 1
 | 0       := []
 | (n + 1) :=
-    if 0 < weight (lambda' n) η υ then
-      if h : (is_exists_inv_infinity (lambda' n) η υ).is_some then
-        sum.inl (option.get h) :: lambda' n
+    if 0 < weight (lambda' n) υ then
+      if h : (is_exists_inv_infinity (lambda' n) υ).is_some then
+        sum.inr (option.get h) :: lambda' n
       else ∞ :: lambda' n
     else lambda' n 
 
-def lambda (η : Tree 0) (υ : subTree η → option (Tree 1)) : Tree 1 := lambda' η υ η.length
+def lambda {η : Tree 0} (υ : subTree η → option (Tree 1)) : Tree 1 := lambda' υ η.length
 
-def assign (η : Tree 0) (υ : subTree η → option (Tree 1)) : Tree 1 → option (Tree 1 × ℕ)
+def assign {η : Tree 0} (υ : subTree η → option (Tree 1)) : Tree 1 → option (Tree 1 × ℕ)
 | []               := none
-| (sum.inl _ :: μ) := assign μ
 | (∞ :: μ)        :=
-  if h : (assign μ).is_some then S.inf (option.get h) (μ, weight μ η υ) else
-  some (μ, weight μ η υ)
+  if h : (assign μ).is_some then S.inf (option.get h) (μ, weight μ υ) else
+  some (μ, weight μ υ)
+| (sum.inr _ :: μ) := assign μ
 
-def assign_eq (η : Tree 0) (υ : subTree η → option (Tree 1)) : Tree 1 → option (Tree 1 × ℕ) := λ μ,
-if h : (assign S η υ μ).is_some then S.inf (option.get h) (μ, weight μ η υ) else
-  some (μ, weight μ η υ)
 
-def up (η : Tree 0) (υ : subTree η → option (Tree 1)) : option (Tree 1 × ℕ) := assign_eq S η υ (lambda η υ)
+def assign_eq {η : Tree 0} (υ : subTree η → option (Tree 1)) : Tree 1 → option (Tree 1 × ℕ) := λ μ, assign S υ (∞ :: μ)
 
-def requirement (η : Tree 0) (υ : subTree η → option (Tree 1)) : option R := (up S η υ).map S.requirement
+def assignment {η : Tree 0} (υ : subTree η → option (Tree 1)) : option (Tree 1 × ℕ) := assign_eq S υ (lambda υ)
+
+def up {η : Tree 0} (υ : subTree η → option (Tree 1)) : option (Tree 1) := (assignment S υ).map prod.fst
+
+def requirement {η : Tree 0} (υ : subTree η → option (Tree 1)) : option R := (assignment S υ).map S.requirement
 
 end approx
 
-mutual def weight, is_exists_inv_infinity, lambda', assign, up
-with weight : Tree 0 → Tree 1 → ℕ
-| []       _ := 0
-| (_ :: η) μ := weight η μ + (if (up η).map prod.fst = ↑μ then 1 else 0)
+def up' (S : strategy R) : ∀ (η : Tree 0) (μ : subTree η), option (Tree 1)
+| []       ⟨μ, μ_p⟩ := by exfalso; simp* at*
+| (_ :: η) ⟨μ, μ_p₁, μ_p₂⟩ :=
+    have lmm : μ <:+ η,
+    { have := list.suffix_cons_iff.mp μ_p₁, cases this,
+      { exfalso, exact μ_p₂ this }, { exact this } },
+    if h : μ = η then approx.up S (up' η) else up' η ⟨μ, lmm, h⟩
 
-with is_exists_inv_infinity : Tree 0 → Tree 1 → option (Tree 0)
-| []               _ := none
-| (sum.inl _ :: η) μ := is_exists_inv_infinity η μ
-| (∞ :: η)        μ :=
-    if (is_exists_inv_infinity η μ).is_some then is_exists_inv_infinity η μ
-    else if (up η).map prod.fst = ↑μ then some η else none
+def up (η : Tree 0) : option (Tree 1) := approx.up S (up' S η)
 
-with lambda' : ℕ → Tree 0 → Tree 1
-| 0       _ := []
-| (n + 1) η :=
-    if 0 < weight η (lambda' n η) then
-      if h : (is_exists_inv_infinity η (lambda' n η)).is_some then
-        sum.inl (option.get h) :: lambda' n η
-      else ∞ :: lambda' n η
-    else lambda' n η
+lemma up'_up_consistent {η : Tree 0} : ∀ (μ : subTree η), S.up' η μ = S.up μ.val :=
+begin
+  induction η with ν η IH,
+  { intros μ, have := μ.property, simp* at* },
+  { intros μ, cases μ with μ μ_p, rcases μ_p with ⟨μ_p₁, μ_p₂⟩, simp[up', up],
+    by_cases C : μ = η; simp[C], { rw [C] }, { simp[IH], refl } }
+end
 
-with assign : Tree 0 → Tree 1 → option (Tree 1 × ℕ)
-| η []               := none
-| η (sum.inl _ :: μ) := assign η μ
-| η (∞ :: μ)        :=
-  if h : (assign η μ).is_some then S.inf (option.get h) (μ, weight η μ) else
-  some (μ, weight η μ)
+def lambda (η : Tree 0) : Tree 1 := approx.lambda (up' S η)
 
-with up : Tree 0 → option (Tree 1 × ℕ)
-| η := 
-  let
-    assign : Tree 0 → Tree 1 → option (Tree 1 × ℕ) := λ η μ,
-      match μ with
-      | []               := none
-      | (sum.inl _ :: μ) := assign η μ
-      | (∞ :: μ)        := none end,
-    lambda (η : Tree 0) : Tree 1 := lambda' η.length η,
-    assign_eq (η : Tree 0) : Tree 1 → option (Tree 1 × ℕ) := λ μ,
-      if h : (assign η μ).is_some then S.inf (option.get h) (μ, weight η μ) else
-      some (μ, weight η μ) in
-  assign_eq η (lambda η)
+def assignment (η : Tree 0) : option (Tree 1 × ℕ) := approx.assignment S (up' S η)
+#check up
+
+@[simp] lemma lambda_nil : S.lambda [] = [] := rfl
+
+lemma is_exists_inv_infinity_infinity (η : Tree 1) (μ : Tree 0) (μ₀ : Tree 0)
+  (h1 : out[μ] μ₀ ↝ ∞) (h2 : S.up μ₀ = η) : out[S.lambda μ] η ↝ sum.inr μ₀ :=
+begin
+  induction μ with ν μ IH μ IH generalizing μ₀,
+  simp,
+end
+
+
+variables (Λ : Tree_path 0)
+
+theorem finite_injury :
+  ∀ (n : ℕ), ∃ (s₀ : ℕ), ∀ (s : ℕ), s₀ ≤ s →
+    S.lambda (Λ.path s)↾*n = S.lambda (Λ.path s₀)↾*n := λ n,
+begin
+  induction n with n IH,
+  { simp },
+  { rcases IH with ⟨s₀, IH⟩,
+    suffices :
+      ∃ s₁, s₀ ≤ s₁ ∧ ∀ s, s₁ ≤ s → (S.lambda (Λ.path s)).rnth n = (S.lambda (Λ.path s₁)).rnth n,
+    { rcases this with ⟨s₁, eqn, hyp_s₁⟩, refine ⟨s₁, λ s eqn_s, _⟩,
+      apply list.rnth_ext', { intros m a, simp[list.initial_rnth_some_iff], sorry } },
+    by_cases C₁ : ∀ s, list.rnth (S.lambda (Λ.path s)) n = none,
+    { refine ⟨s₀, by refl, λ s eqn_s, _⟩, simp[C₁] },
+    have C₁ : ∃ (s₁ : ℕ) (ν : infinity ⊕ Tree 0), list.rnth (S.lambda (Λ.path s₁)) n = some ν,
+    { simp at C₁, rcases C₁ with ⟨s₁, C₁⟩, have := option.ne_none_iff_exists'.mp C₁, exact ⟨s₁, this⟩ },
+    rcases C₁ with ⟨s₁, ν, C₁⟩,
+    cases ν,
+    { cases ν, refine ⟨max s₀ s₁, by simp, λ s eqn_s, _⟩,
+        } }
+
+end 
 
 end strategy
 
